Protocols/ABC/OldProofs/Invariant.v
@@ -4,14 +4,15 @@ Import (coercions) ssrbool.
 Import ssreflect.SsrSyntax.
 From ABCProtocol.Protocols.ABC.OldProofs Require Export Network.
 
-Module ACInvariant (A : NetAddr) (V : Signable) (VBFT : ValueBFT A V) 
+Module ACInvariant (A : NetAddr) (Sn : Signable) (V : Value Sn) (VBFT : ValueBFT A Sn V) 
   (BTh : ByzThreshold A) (BSett : ByzSetting A)
-  (P : PKI A V) (TSS : ThresholdSignatureScheme A V with Definition thres := BTh.t0).
+  (P : PKI A Sn) (TSS0 : ThresholdSignatureSchemePrim A Sn with Definition thres := BTh.t0) (* ! *)
+  (TSS : ThresholdSignatureScheme A Sn with Module TSSPrim := TSS0).
 
 Import A V VBFT BTh BSett P TSS.
 Import ssrbool. (* anyway *)
 
-Module Export ACN := ACNetwork A V VBFT BTh BSett P TSS.
+Module Export ACN := ACNetwork A Sn V VBFT BTh BSett P TSS0 TSS.
 
 (* this is somewhat "pure" property (not related to psent) *)
 (* HMM why there is not something like "if confirmed, then submitted"?
