Protocols/RB/Types.v
@@ -11,6 +11,14 @@ Parameter inputval : Value. (* to be broadcast *)
 End Leadership.
 *)
 
+Module Type Value.
+
+(* here, only requires that value has decidable equality *)
+Parameter Value : Set.
+Parameter Value_eqdec : forall (v1 v2 : Value), {v1 = v2} + {v1 <> v2}.
+
+End Value.
+
 Module Type RBTag.
 
 Parameter Round : Type.
@@ -18,7 +26,7 @@ Parameter Round_eqdec : forall r1 r2 : Round, {r1 = r2} + {r1 <> r2}.
 
 End RBTag.
 
-Module Type ValueBFT (Export A : NetAddr) (Export R : RBTag) (Export V : Signable).
+Module Type ValueBFT (Export A : NetAddr) (Export R : RBTag) (Export V : Value).
 
 (* fixing what to broadcast at each round *)
 
@@ -27,7 +35,7 @@ Parameter value_bft : Address -> Round -> Value.
 End ValueBFT.
 
 Module Type RBMessage (A : NetAddr) (R : RBTag)
-  (V : Signable (* not for signing here, though *)) <: MessageType.
+  (V : Value (* not for signing here, though *)) <: MessageType.
 
 Import A R V.
 
@@ -46,7 +54,7 @@ Qed.
 
 End RBMessage.
 
-Module RBMessageImpl (A : NetAddr) (R : RBTag) (V : Signable) <: MessageType <: RBMessage A R V.
+Module RBMessageImpl (A : NetAddr) (R : RBTag) (V : Value) <: MessageType <: RBMessage A R V.
 
 Include RBMessage A R V.
 
